Proofs/AES-GCM/GCMInitV8Sym.lean
@@ -11,11 +11,12 @@ import Specs.GCMV8
 
 namespace GCMInitV8Program
 
+set_option bv.ac_nf false
+
 abbrev H_addr (s : ArmState) : BitVec 64 := r (StateField.GPR 1#5) s
 abbrev Htable_addr (s : ArmState) : BitVec 64 := r (StateField.GPR 0#5) s
 
--- set_option debug.byAsSorry true in
-set_option maxRecDepth 1000000 in
+set_option maxRecDepth 8000 in
 -- set_option profiler true in
 theorem gcm_init_v8_program_run_152 (s0 sf : ArmState)
     (h_s0_program : s0.program = gcm_init_v8_program)
@@ -33,8 +34,13 @@ theorem gcm_init_v8_program_run_152 (s0 sf : ArmState)
   sym_n 152
   done
 
-set_option maxRecDepth 1000000 in
-set_option maxHeartbeats 2000000 in
+set_option maxRecDepth 100000 in
+set_option maxHeartbeats 500000 in
+set_option sat.timeout 120 in
+-- set_option pp.deepTerms true in
+-- set_option pp.maxSteps 10000 in
+-- set_option trace.profiler true in
+-- set_option linter.unusedVariables false in
 -- set_option profiler true in
 theorem gcm_init_v8_program_correct (s0 sf : ArmState)
     (h_s0_program : s0.program = gcm_init_v8_program)
@@ -42,7 +48,7 @@ theorem gcm_init_v8_program_correct (s0 sf : ArmState)
     (h_s0_pc : read_pc s0 = gcm_init_v8_program.min)
     (h_s0_sp_aligned : CheckSPAlignment s0)
     (h_run : sf = run gcm_init_v8_program.length s0)
-    (_h_mem : Memory.Region.pairwiseSeparate
+    (h_mem : Memory.Region.pairwiseSeparate
       [ ⟨(H_addr s0), 128⟩,
         ⟨(Htable_addr s0), 2048⟩ ])
     : -- effects
@@ -59,8 +65,10 @@ theorem gcm_init_v8_program_correct (s0 sf : ArmState)
     -- H_addr ptr stays the same
     ∧ H_addr sf = H_addr s0
     -- v20 - v31 stores results of Htable
-    ∧ read_sfp 128 20#5 sf = (GCMV8.GCMInitV8 (read_mem_bytes 16 (H_addr s0) s0)).get! 0
-    -- ∧ read_sfp 128 21#5 sf = (GCMV8.GCMInitV8 (read_mem_bytes 16 (H_addr s0) s0)).get! 1
+    ∧ let Hinit := (read_mem_bytes 16 (H_addr s0) s0)
+      read_sfp 128 20#5 sf =
+      (GCMV8.GCMInitV8 ((BitVec.extractLsb' 0 64 Hinit) ++ (BitVec.extractLsb' 64 64 Hinit))).get! 0
+    --
     -- TODO: Commenting out memory related conjuncts since it seems
     -- to make symbolic execution stuck
     --   -- First 12 elements in Htable is correct
@@ -73,6 +81,7 @@ theorem gcm_init_v8_program_correct (s0 sf : ArmState)
     -- ∧ (∀ (f : StateField), ¬ (f = StateField.PC) ∧
     --                        ¬ (f = (StateField.GPR 29#5)) →
     --     r f sf = r f s0)
+    --
     -- -- Memory safety: memory location that should not change did
     -- -- not change
     -- -- The addr exclude output region Htable
@@ -84,6 +93,32 @@ theorem gcm_init_v8_program_correct (s0 sf : ArmState)
   --    unable to be reflected
   sym_n 152
   simp only [Htable_addr, state_value] -- TODO: state_value is needed, why
-  apply And.intro
+  apply And.intro  
   · bv_decide
   · sorry
+  -- [Shilpi] Commenting out the following because the CI fails with 
+  -- "INTERNAL PANIC: out of memory"
+  /-
+    simp only
+    [shift_left_common_aux_64_2
+    , shift_right_common_aux_64_2_tff
+    , shift_right_common_aux_32_4_fff
+    , DPSFP.AdvSIMDExpandImm
+    , DPSFP.dup_aux_0_4_32]
+    generalize read_mem_bytes 16 (r (StateField.GPR 1#5) s0) s0 = Hinit
+    -- change the type of Hinit to be BitVec 128, assuming that's def-eq
+    change BitVec 128 at Hinit
+    simp only [GCMV8.GCMInitV8, GCMV8.lo, List.get!, GCMV8.hi,
+      GCMV8.gcm_init_H, GCMV8.refpoly, GCMV8.pmod, GCMV8.pmod.pmodTR,
+      GCMV8.reduce, GCMV8.degree, GCMV8.degree.degreeTR]
+    simp only [Nat.reduceAdd, BitVec.ushiftRight_eq, BitVec.reduceExtracLsb',
+      BitVec.reduceHShiftLeft, BitVec.reduceAppend, BitVec.reduceHShiftRight, BitVec.ofNat_eq_ofNat,
+      BitVec.reduceEq, ↓reduceIte, BitVec.zero_eq, Nat.sub_self, BitVec.ushiftRight_zero_eq,
+      BitVec.reduceAnd, BitVec.toNat_ofNat, Nat.pow_one, Nat.reduceMod, Nat.mul_zero, Nat.add_zero,
+      Nat.zero_mod, Nat.zero_add, Nat.sub_zero, Nat.mul_one, Nat.zero_mul, Nat.one_mul,
+      Nat.reduceSub, BitVec.reduceMul, BitVec.reduceXOr, BitVec.mul_one, Nat.add_one_sub_one,
+      BitVec.one_mul]
+    -- bv_check "GCMInitV8Sym.lean-GCMInitV8Program.gcm_init_v8_program_correct-117-4.lrat"
+    -- TODO: proof works in vscode but timeout in the CI -- need to investigate further
+    -/
+
